Expanding on parametric forcing.

theories/reader/ForcingParam.v
@@ -45,6 +45,10 @@ Definition Typeᴿ p (A : Typeᵒ p) := {
         Aε r (β ∘ α) (fun s γ => x s (γ ∘ β))
 }.
 
+Definition TYPE p := {A : Typeᵒ p & Typeᴿ p A}.
+Definition El p (A : TYPE p) :=
+  { x : forall (q : Ω) (α : Θ q p), A.(fst) q α & A.(snd).(fst) p (refl p) x }.
+
 Definition Typeᶱ : forall p (A : Typeᵒ p) (Aε : Typeᴿ p A) q (α : Θ q p),
   Typeᴿ q (fun r β => A r (β ∘ α)).
 Proof.
@@ -52,6 +56,26 @@ unshelve refine (fun p A Aε q α => exist _ _ _ _).
 + refine (fun r β x => Aε.(fst) r (β ∘ α) x).
 + refine (fun r β x xε s γ => _).
   refine (Aε.(snd) r (β ∘ α) x xε s γ).
+Defined.
+
+Definition Type0 p : TYPE p.
+Proof.
+unshelve refine (
+  exist (Typeᵒ p) (Typeᴿ p) (fun q α => Type) (exist _ _ (fun q α => Typeᴿ q) _)
+).
+refine (fun q α A Aε r β => Typeᶱ q A Aε r β).
+Defined.
+
+Definition Typeᶠ p : El p (Type0 p) := Type0 p.
+
+Definition TYPEᶱ p (A : TYPE p) q (α : Θ q p) : TYPE q :=
+  exist (Typeᵒ q) (Typeᴿ q) (fun r β => A.(fst) r (β ∘ α)) (Typeᶱ p A.(fst) A.(snd) q α).
+
+Definition θ {p} {A : TYPE p} (x : El p A) {q} (α : Θ q p) : El q (TYPEᶱ p A q α).
+Proof.
+unshelve refine (exist _ _ _ _).
++ refine (fun r β => x.(fst) r (β ∘ α)).
++ refine (A.(snd).(snd) p (refl p) x.(fst) x.(snd) q α).
 Defined.
 
 Goal forall (p : Ω),
@@ -85,3 +109,248 @@ refine (
   fun A Aε x xε => xε
 ).
 Defined.
+
+Definition Arrowᵒ p (q : Ω) (α : Θ q p) (A : TYPE q) (B : TYPE q) : Type :=
+  forall x : El q A, B.(fst) q (refl q).
+
+Definition Arrowᴿ p (q : Ω) (α : Θ q p) (A : TYPE q) (B : TYPE q) :
+  Typeᴿ q (fun r β => Arrowᵒ p r (β ∘ α) (TYPEᶱ q A r β) (TYPEᶱ q B r β)).
+Proof.
+unshelve refine (exist _ _ _ _); cbn in *.
+  - unshelve refine
+    (fun r β f =>
+      forall
+        (s : Ω) (γ : Θ s r) (x : El s (TYPEᶱ q A s (γ ∘ β))),
+        B.(snd).(fst) s (γ ∘ β) (fun t δ => f t (δ ∘ γ) (θ x δ))
+    ).
+  - unshelve refine (fun r β f fε s γ t δ x => fε _ _ _).
+Defined.
+
+Definition Arrow0 p (A : El p (Typeᶠ p)) (B : El p (Typeᶠ p)) : El p (Typeᶠ p).
+Proof.
+unshelve refine (exist _ _ _ _).
++ refine (fun q α => Arrowᵒ p q α (θ A α) (θ B α)).
++ refine (Arrowᴿ p p (refl p) A B).
+Defined.
+
+(*
+Definition Arrowᶠ p :
+  { T :
+    forall (q : Ω) (α : Θ q p)
+    (A : TYPE q)
+    (B : TYPE q),
+    Type
+  & forall (q : Ω) (α : Θ q p)
+    (A : TYPE q)
+    (B : TYPE q),
+    Typeᴿ q (fun r β => T r (β ∘ α) (TYPEᶱ q A r β) (TYPEᶱ q B r β)) }
+.
+Proof.
+unshelve refine (exist _ _ _ _).
++ refine (Arrowᵒ p).
++ refine (fun q α => Arrowᴿ q q (refl _)).
+Defined.*)
+
+(* Notation "A →ᶠ B" := (Arrowᶠ A (fun _ => B)) (at level 99, right associativity, B at level 200). *)
+
+
+(* Check (fun p => Arrowᶠ p) : forall p, El p (Arrowᶠ p Typeᶠ. *)
+
+(**
+
+Definition Arrowᵒ p
+  (q : Ω) (α : Θ q p)
+  (A : Typeᵒ q)
+  (Aε : Typeᴿ q A)
+  (B : Typeᵒ q)
+  (Bε : Typeᴿ q B)
+  : Type.
+Proof.
+refine (
+  forall
+    (x : (forall r (β : Θ r q), A r β))
+    (xε : Aε.(fst) q (refl q) x),
+    B q (refl q)
+).
+Defined.
+
+
+Definition Arrowᴿ p
+  (q : Ω) (α : Θ q p)
+  (A : Typeᵒ q)
+  (Aε : Typeᴿ q A)
+  (B : Typeᵒ q)
+  (Bε : Typeᴿ q B)
+  : Typeᴿ q (fun r β =>
+    Arrowᵒ q r β
+      (fun s γ => A s (γ ∘ β))
+      (Typeᶱ _ A Aε _ _)
+      (fun s γ => B s (γ ∘ β))
+      (Typeᶱ _ B Bε _ _)
+  ).
+Proof.
+unshelve refine (exist _ _ _ _); unfold Arrowᵒ; cbn in *.
++ unshelve refine
+  (fun r β f =>
+    forall
+      (s : Ω) (γ : Θ s r)
+      (x : (forall t δ, A t (δ ∘ γ ∘ β)))
+      (xε : Aε.(fst) s (γ ∘ β) x),
+      Bε.(fst) s (γ ∘ β)
+        (fun t δ => f t (δ ∘ γ) (fun u ε => x u (ε ∘ δ)) (Aε.(snd) s (γ ∘ β) x xε t δ))
+  ).
++ unshelve refine (fun r β f fε s γ t δ x xε => fε _ _ _ _).
+Defined.
+
+Definition Prodᵒ p
+  (q : Ω) (α : Θ q p)
+  (A : Typeᵒ q)
+  (Aε : Typeᴿ q A)
+  (B : forall (r : Ω) (β : Θ r q)
+    (x : forall (s : Ω) (γ : Θ s r), A s (γ ∘ β))
+    (xε : Aε.(fst) r _ x), Type)
+  (Bε : forall (r : Ω) (β : Θ r q)
+    (x : forall (s : Ω) (γ : Θ s r), A s (γ ∘ β))
+    (xε : Aε.(fst) r β x),
+      Typeᴿ r (fun s γ => B s (γ ∘ β) (fun t δ => x t (δ ∘ γ)) (Aε.(snd) _ _ x xε _ _)))
+  : Type.
+Proof.
+refine (
+  forall
+    (x : (forall r (β : Θ r q), A r β))
+    (xε : Aε.(fst) q (refl q) x),
+    B _ (refl _) x xε
+).
+Defined.
+
+Definition Prodᴿ p
+  (q : Ω) (α : Θ q p)
+  (A : Typeᵒ q)
+  (Aε : Typeᴿ q A)
+  (B : forall (r : Ω) (β : Θ r q)
+    (x : forall (s : Ω) (γ : Θ s r), A s (γ ∘ β))
+    (xε : Aε.(fst) r _ x), Type)
+  (Bε : forall (r : Ω) (β : Θ r q)
+    (x : forall (s : Ω) (γ : Θ s r), A s (γ ∘ β))
+    (xε : Aε.(fst) r β x),
+      Typeᴿ r (fun s γ => B s (γ ∘ β) (fun t δ => x t (δ ∘ γ)) (Aε.(snd) _ _ x xε _ _)))
+  :
+  Typeᴿ q (fun r γ =>
+      Prodᵒ q r γ
+        (fun s δ => A s (δ ∘ γ))
+        (Typeᶱ _ _ Aε _ _)
+        (fun s δ x xε => B s (δ ∘ γ) x xε)
+        (fun s δ x xε => Bε _ _ x xε)
+    ).
+Proof.
+unshelve refine (exist _ _ _ _).
++ unshelve refine (
+  fun r γ f =>
+    forall
+      (x : (forall s δ, A s (δ ∘ γ)))
+      (xε : Aε.(fst) _ _ x),
+      (Bε _ _ x xε).(fst) r (refl r)
+        (fun s δ => f s _
+          (fun t ε => x t (ε ∘ δ))
+          (Aε.(snd) _ _ x xε _ _)
+        )
+).
++ unshelve refine (
+    fun r γ f fε s δ x xε => _
+  ).
+cbn in *.
+Abort.
+
+*)
+
+Inductive unitᵒ (p : Ω) := ttᵒ.
+Inductive unitε (p : Ω) : (forall q (α : Θ q p), unitᵒ q) -> Type :=
+| ttε : unitε p (fun q _ => ttᵒ q).
+
+Definition unitᴿ p : Typeᴿ p (fun q α => unitᵒ q).
+Proof.
+unshelve refine (exist _ _ _ _).
++ refine (fun q α => unitε q).
++ unshelve refine (fun q α i iε r β => _).
+  destruct iε; constructor.
+Defined.
+
+Definition unit_indᵒ
+  (p : Ω)
+  (q : Ω) (α : Θ q p)
+  (P : forall r (β : Θ r q)
+    (i : forall s (γ : Θ s r), unitᵒ s)
+    (iε : (unitᴿ r).(fst) r (refl r) i),
+    Type)
+  (Pε : forall
+    (i : forall r (β : Θ r q), unitᵒ r)
+    (iε : (unitᴿ q).(fst) q (refl _) i),
+    Typeᴿ q (fun r β =>
+      P r β
+        (fun s γ => i s (γ ∘ β))
+        ((unitᴿ q).(snd) _ (refl q) i iε _ β)
+    )
+  )
+  (π : forall r (β : Θ r q), P r β (fun s γ => ttᵒ s) (ttε r))
+  (πε : (Pε (fun r β => ttᵒ r) (ttε q)).(fst) q (refl q) π)
+  (i : forall r (β : Θ r q), unitᵒ r)
+  (iε : (unitᴿ q).(fst) q (refl q) i) :
+  P q (refl q) i iε.
+Proof.
+refine (
+  match iε in unitε _ i return P q (refl q) i iε with
+  | ttε _ => π _ _
+  end
+).
+Defined.
+
+(* Definition unit_indᴿ *)
+Goal Type.
+unshelve refine (forall
+  (p : Ω)
+  (q : Ω) (α : Θ q p)
+  (P : forall r (β : Θ r q)
+    (i : forall s (γ : Θ s r), unitᵒ s)
+    (iε : (unitᴿ r).(fst) r (refl r) i),
+    Type)
+  (Pε : forall
+    (i : forall r (β : Θ r q), unitᵒ r)
+    (iε : (unitᴿ q).(fst) q (refl _) i),
+    Typeᴿ q (fun r β =>
+      P r β
+        (fun s γ => i s (γ ∘ β))
+        ((unitᴿ q).(snd) _ (refl q) i iε _ β)
+    )
+  )
+  (π : forall r (β : Θ r q), P r β (fun s γ => ttᵒ s) (ttε r))
+  (πε : (Pε (fun r β => ttᵒ r) (ttε q)).(fst) q (refl q) π)
+  (i : forall r (β : Θ r q), unitᵒ r)
+  (iε : (unitᴿ q).(fst) q (refl q) i)
+  ,
+  (Pε i iε).(fst) q (refl q)
+    (fun r β =>
+      unit_indᵒ q r β
+        (fun s γ i iε => P s (γ ∘ β) i iε)
+        (fun i iε => _)
+        (fun s γ => π s (γ ∘ β))
+        _
+        (fun s γ => i s (γ ∘ β))
+        ((unitᴿ q).(snd) q (refl q) i iε r β)
+  )).
+
+
+cbn in *.
+pose (unitᴿ r).(snd).
+cbn in *.
+
+refine (let X := Typeᶱ q (fun r β => P r β (fun s γ => i s (γ ∘ β)) _) in _).
+
+
+pose (Typeᶱ r (fun s γ =>
+  P s (γ ∘ β)
+    (fun t δ => i t (δ ∘ γ))
+    ((unitᴿ r).(snd) r (refl r) i iε _ _)
+)).
+cbn in *.
+refine (Typeᶱ q (fun s γ => P s γ _ _) _ r β).
+refine (Pε _ _).
